Lean4Lean/Verify/Typing/Lemmas.lean
@@ -1,9 +1,11 @@
+import Std.Data.String.Lemmas
 import Lean4Lean.Verify.Typing.Expr
 import Lean4Lean.Theory.Typing.Strong
 import Lean4Lean.Theory.Typing.UniqueTyping
 
 namespace Lean4Lean
 open VEnv Lean
+open scoped List
 
 theorem InScope.mono {P Q : FVarId → Prop} (H : ∀ fv, P fv → Q fv) :
     ∀ {e k}, InScope P e k → InScope Q e k
@@ -15,8 +17,22 @@ theorem InScope.mono {P Q : FVarId → Prop} (H : ∀ fv, P fv → Q fv) :
   | .letE .., _, ⟨h1, h2, h3⟩ => ⟨h1.mono H, h2.mono H, h3.mono H⟩
   | .proj _ _ e, _, h | .mdata _ e, _, h => h.mono (e := e) H
 
-theorem VLocalDecl.WF.hasType :
-    ∀ {d}, VLocalDecl.WF env U Δ d → env.HasType U (VLCtx.toCtx ((ofv, d) :: Δ)) d.value d.type
+theorem InScope.natLitToConstructor : InScope P (.natLitToConstructor n) k := by
+  cases n <;> simp [InScope]
+
+theorem InScope.strLitToConstructor : InScope P (.strLitToConstructor s) k := by
+  simp [InScope, String.foldr_eq]; induction s.data <;> simp [*, InScope]
+
+theorem InScope.toConstructor : ∀ {l : Literal}, InScope P l.toConstructor k
+  | .natVal _ => .natLitToConstructor
+  | .strVal _ => .strLitToConstructor
+
+theorem InScope.fvars_cons :
+    InScope (· ∈ VLCtx.fvars Δ) e k → InScope (· ∈ VLCtx.fvars ((ofv, d) :: Δ)) e k :=
+  InScope.mono fun a h => by cases ofv <;> simp [h]
+
+theorem VLocalDecl.WF.hasType : ∀ {d}, VLocalDecl.WF env U (VLCtx.toCtx Δ) d →
+    env.HasType U (VLCtx.toCtx ((ofv, d) :: Δ)) d.value d.type
   | .vlam _, _ => .bvar .zero
   | .vlet .., hA => hA
 
@@ -24,6 +40,19 @@ theorem VLocalDecl.is_liftN {Δ : VLCtx} :
     ∀ {d}, Ctx.LiftN (VLocalDecl.depth d) 0 Δ.toCtx (VLCtx.toCtx ((ofv, d) :: Δ))
   | .vlam _ => .one
   | .vlet .. => .zero []
+
+variable (env : VEnv) (U : Nat) (Γ : List VExpr) in
+inductive VLocalDecl.IsDefEq : VLocalDecl → VLocalDecl → Prop
+  | vlam : env.IsDefEq U Γ type₁ type₂ (.sort u) → VLocalDecl.IsDefEq (.vlam type₁) (.vlam type₂)
+  | vlet :
+    env.IsDefEq U Γ value₁ value₂ type₁ → env.IsDefEq U Γ type₁ type₂ (.sort u) →
+    VLocalDecl.IsDefEq (.vlet type₁ value₁) (.vlet type₂ value₂)
+
+variable (henv : Ordered env) (hΓ' : OnCtx Γ' (env.IsType U)) (W : Ctx.LiftN n k Γ Γ') in
+theorem VLocalDecl.weakN_iff : VLocalDecl.WF env U Γ' (d.liftN n k) ↔ VLocalDecl.WF env U Γ d :=
+  match d with
+  | .vlam .. => IsType.weakN_iff henv hΓ' W
+  | .vlet .. => HasType.weakN_iff henv hΓ' W
 
 variable (henv : Ordered env) in
 theorem VLCtx.WF.find?_wf {Δ : VLCtx} (hΔ : VLCtx.WF env U Δ) (H : Δ.find? v = some (e, A)) :
@@ -41,43 +70,149 @@ theorem VLCtx.WF.toCtx : ∀ {Δ}, VLCtx.WF env U Δ → OnCtx Δ.toCtx (env.IsT
   | (_, .vlam _) :: _, ⟨hΔ, _, hA⟩ => ⟨hΔ.toCtx, hA⟩
   | (_, .vlet ..) :: _, ⟨hΔ, _, _⟩ => hΔ.toCtx
 
+theorem VLCtx.WF.fvars_nodup : ∀ {Δ}, VLCtx.WF env U Δ → Δ.fvars.Nodup
+  | [], _ => .nil
+  | (none, _) :: Δ, ⟨hΔ, _, _⟩ => fvars_nodup (Δ := Δ) hΔ
+  | (some fv, _) :: Δ, ⟨hΔ,  h, _⟩ => by
+    suffices fv ∉ fvars Δ from (fvars_nodup hΔ).cons (fun _ h e => this (e ▸ h))
+    simp [bind] at h
+    simpa only [mem_fvars, ← Option.isSome_iff_exists, Option.not_isSome_iff_eq_none] using h
+
+namespace VLCtx
+
+inductive LiftN : VLCtx → VLCtx → Nat → Nat → Nat → Prop
+  | refl : LiftN Δ Δ 0 0 0
+  | skip_fvar (fv d) : LiftN Δ Δ' 0 n 0 → LiftN Δ ((some fv, d) :: Δ') 0 (n + d.depth) 0
+  | cons_bvar (d) : LiftN Δ Δ' dk n k →
+    LiftN ((none, d) :: Δ) ((none, d.liftN n k) :: Δ') (dk + 1) n (k + d.depth)
+
+theorem LiftN.toCtx (W : LiftN Δ Δ' dk n k) : Ctx.LiftN n k Δ.toCtx Δ'.toCtx := by
+  induction W with
+  | refl => exact .zero []
+  | @skip_fvar _ Δ' _ _ d _ ih =>
+    match d with
+    | .vlet .. => exact ih
+    | .vlam A =>
+      generalize hΓ' : VLCtx.toCtx Δ' = Γ' at ih
+      let .zero As eq := ih
+      simp [VLCtx.toCtx, hΓ']
+      exact .zero (A :: As) (eq ▸ rfl)
+  | cons_bvar d _ ih =>
+    match d with
+    | .vlet .. => exact ih
+    | .vlam A => exact .succ ih
+
+variable (henv : Ordered env) in
+theorem LiftN.wf (W : LiftN Δ Δ' dk n k) (hΔ' : Δ'.WF env U) : Δ.WF env U := by
+  induction W with
+  | refl => exact hΔ'
+  | skip_fvar _ _ _ ih => exact ih hΔ'.1
+  | cons_bvar _ W ih =>
+    let ⟨hΔ', _, h2⟩ := hΔ'
+    exact ⟨ih hΔ', rfl, (VLocalDecl.weakN_iff henv hΔ'.toCtx W.toCtx).1 h2⟩
+
+variable (henv : Ordered env) in
+theorem LiftN.fvars_suffix (W : LiftN Δ Δ' dk n k) : Δ.fvars <:+ Δ'.fvars := by
+  induction W with
+  | refl => exact List.suffix_refl _
+  | skip_fvar _ _ _ ih => exact ih.trans (List.suffix_cons ..)
+  | cons_bvar _ _ ih => exact ih
+
+theorem LiftN.find? (W : VLCtx.LiftN Δ Δ' dk n k) (hΔ' : Δ'.WF env U)
+    (H : VLCtx.find? Δ v = some (e, A)) : VLCtx.find? Δ' v = some (e.liftN n k, A.liftN n k) := by
+  induction W generalizing v e A with
+  | refl => simp [H]
+  | @skip_fvar _ Δ' _ fv' _ W ih =>
+    simp [VLCtx.find?]
+    cases v with simp [VLCtx.next, bind]
+    | inl => exact ⟨_, ih hΔ'.1 H, by simp [VExpr.liftN_liftN]⟩
+    | inr fv =>
+      cases eq : fv' == fv <;> simp
+      · exact ⟨_, ih hΔ'.1 H, by simp [VExpr.liftN_liftN]⟩
+      · refine ((List.pairwise_cons.1 hΔ'.fvars_nodup).1 fv' ?_ rfl).elim
+        refine W.fvars_suffix.subset (mem_fvars.2 ?_)
+        rw [← Option.isSome_iff_exists, lookup_isSome, (beq_iff_eq ..).1 eq]
+        exact Option.isSome_iff_exists.2 ⟨_, H⟩
+  | cons_bvar d _ ih =>
+    simp [VLCtx.find?] at H ⊢
+    obtain ⟨_|i⟩ | fv := v <;> simp [VLCtx.next, bind] at H ⊢ <;>
+      [(obtain ⟨rfl, rfl⟩ := H);
+       (obtain ⟨⟨e, A⟩, H, rfl, rfl⟩ := H
+        refine ⟨_, ih (v := .inl i) hΔ'.1 H, ?_⟩);
+       (obtain ⟨⟨e, A⟩, H, rfl, rfl⟩ := H
+        refine ⟨_, ih (v := .inr fv) hΔ'.1 H, ?_⟩)] <;>
+      open VLocalDecl in
+      cases d <;> simp [VExpr.lift_liftN', liftN, value, type, depth, VExpr.liftN]
+
+end VLCtx
+
+theorem TrProj.weakN (W : Ctx.LiftN n k Γ Γ')
+    (H : TrProj Γ s i e e') : TrProj Γ' s i (e'.liftN n k) (e'.liftN n k) := sorry
+
+variable (henv : Ordered env) in
+theorem TrExpr.weakN (W : VLCtx.LiftN Δ Δ' dk n k) (hΔ' : Δ'.WF env Us.length)
+    (H : TrExpr env Us Δ e e') : TrExpr env Us Δ' e (e'.liftN n k) := by
+  induction H generalizing Δ' dk k with
+  | bvar h1 => exact .bvar (W.find? hΔ' h1)
+  | fvar h1 => exact .fvar (W.find? hΔ' h1)
+  | sort h1 => exact .sort h1
+  | const h1 h2 h3 => exact .const h1 h2 h3
+  | app h1 h2 _ _ ih1 ih2 =>
+    exact .app (h1.weakN henv W.toCtx) (h2.weakN henv W.toCtx) (ih1 W hΔ') (ih2 W hΔ')
+  | lam h1 _ _ ih1 ih2 =>
+    have h1 := h1.weakN henv W.toCtx
+    exact .lam h1 (ih1 W hΔ') (ih2 (W.cons_bvar _) ⟨hΔ', rfl, h1⟩)
+  | forallE h1 h2 _ _ ih1 ih2 =>
+    have h1 := h1.weakN henv W.toCtx
+    have h2 := h2.weakN henv W.toCtx.succ
+    exact .forallE h1 h2 (ih1 W hΔ') (ih2 (W.cons_bvar _) ⟨hΔ', rfl, h1⟩)
+  | letE h1 _ _ _ ih1 ih2 ih3 =>
+    have h1 := h1.weakN henv W.toCtx
+    exact .letE h1 (ih1 W hΔ') (ih2 W hΔ') (ih3 (W.cons_bvar _) ⟨hΔ', rfl, h1⟩)
+  | lit _ ih => exact .lit (ih W hΔ')
+  | mdata _ ih => exact .mdata (ih W hΔ')
+  | proj _ h2 ih => exact .proj (ih W hΔ') (h2.weakN W.toCtx)
+
+variable (henv : Ordered env) (hΓ' : OnCtx Γ' (env.IsType U)) in
+theorem HasType.skips (W : Ctx.LiftN n k Γ Γ')
+    (h1 : env.HasType U Γ' e A) (h2 : e.Skips n k) : ∃ B, env.HasType U Γ' e B ∧ B.Skips n k :=
+  IsDefEq.skips henv hΓ' W h1 h2 h2
+
+theorem TrProj.weakN_inv (henv : Ordered env) (hΓ' : OnCtx Γ' (env.IsType U))
+    (W : Ctx.LiftN n k Γ Γ') : TrProj Γ' s i (e.liftN n k) e' → ∃ e', TrProj Γ s i e e' := sorry
+
+theorem TrProj.defeqDFC (henv : Ordered env) (hΓ : env.IsDefEqCtx U [] Γ₁ Γ₂)
+    (he : env.IsDefEqU U Γ₁ e₁ e₂) (H : TrProj Γ₁ s i e₁ e') :
+    ∃ e', TrProj Γ₂ s i e₂ e' := sorry
+
 variable (env : VEnv) (U : Nat) in
 inductive VLCtx.IsDefEq : VLCtx → VLCtx → Prop
   | nil : VLCtx.IsDefEq [] []
-  | vlam {Δ₁ Δ₂ : VLCtx} :
+  | cons {Δ₁ Δ₂ : VLCtx} :
     VLCtx.IsDefEq Δ₁ Δ₂ →
     (do Δ₁.lookup (some (← ofv))) = none →
-    env.IsDefEq U Δ₁.toCtx type₁ type₂ (.sort u) →
-    VLCtx.IsDefEq ((ofv, .vlam type₁) :: Δ₁) ((ofv, .vlam type₂) :: Δ₂)
-  | vlet {Δ₁ Δ₂ : VLCtx} :
-    VLCtx.IsDefEq Δ₁ Δ₂ →
-    (do Δ₁.lookup (some (← ofv))) = none →
-    env.IsDefEq U Δ₁.toCtx value₁ value₂ type₁ →
-    env.IsDefEq U Δ₁.toCtx type₁ type₂ (.sort u) →
-    VLCtx.IsDefEq ((ofv, .vlet type₁ value₁) :: Δ₁) ((ofv, .vlet type₂ value₂) :: Δ₂)
+    VLocalDecl.IsDefEq env U Δ₁.toCtx d₁ d₂ →
+    VLCtx.IsDefEq ((ofv, d₁) :: Δ₁) ((ofv, d₂) :: Δ₂)
+
+variable (henv : Ordered env) (hΓ : OnCtx Γ (IsType env U)) in
+theorem VLocalDecl.IsDefEq.refl : ∀ {d}, VLocalDecl.WF env U Γ d → VLocalDecl.IsDefEq env U Γ d d
+  | .vlam _, ⟨_, h1⟩ => .vlam h1
+  | .vlet .., h1 => let ⟨_, h2⟩ := h1.isType henv hΓ; .vlet h1 h2
 
 variable (henv : Ordered env) in
 theorem VLCtx.IsDefEq.refl : ∀ {Δ}, VLCtx.WF env U Δ → VLCtx.IsDefEq env U Δ Δ
   | [], _ => .nil
-  | (_, .vlam ..) :: _, ⟨h1, h2, _, h3⟩ => .vlam (IsDefEq.refl h1) h2 h3
-  | (_, .vlet ..) :: _, ⟨h1, h2, h3⟩ =>
-    let ⟨_, h4⟩ := h3.isType henv h1.toCtx
-    .vlet (IsDefEq.refl h1) h2 h3 h4
+  | (_, _) :: _, ⟨h1, h2, h3⟩ => .cons (IsDefEq.refl h1) h2 (.refl henv h1.toCtx h3)
 
 theorem VLCtx.IsDefEq.defeqCtx : VLCtx.IsDefEq env U Δ₁ Δ₂ → env.IsDefEqCtx U [] Δ₁.toCtx Δ₂.toCtx
   | .nil => .zero
-  | .vlam h1 _ h3 => .succ h1.defeqCtx h3
-  | .vlet h1 _ _ _ => h1.defeqCtx
+  | .cons h1 _ (.vlam h2) => .succ h1.defeqCtx h2
+  | .cons h1 _ (.vlet ..) => h1.defeqCtx
 
 theorem VLCtx.IsDefEq.lookup_eq_none :
     VLCtx.IsDefEq env U Δ₁ Δ₂ → (Δ₁.lookup fv = none ↔ Δ₂.lookup fv = none)
   | .nil => by simp
-  | .vlam h1 _ _ | .vlet h1 _ _ _ => by simp [List.lookup]; split <;> simp [h1.lookup_eq_none]
-
-theorem VLCtx.IsDefEq.find? :
-    VLCtx.IsDefEq env U Δ₁ Δ₂ → (Δ₁.lookup fv = none ↔ Δ₂.lookup fv = none)
-  | .nil => by simp
-  | .vlam h1 _ _ | .vlet h1 _ _ _ => by simp [List.lookup]; split <;> simp [h1.lookup_eq_none]
+  | .cons h1 _ _ => by simp [List.lookup]; split <;> simp [h1.lookup_eq_none]
 
 theorem VLCtx.IsDefEq.bind_lookup_eq_none (H : VLCtx.IsDefEq env U Δ₁ Δ₂) :
     (do Δ₁.lookup (some (← ofv))) = none ↔ (do Δ₂.lookup (some (← ofv))) = none := by
@@ -85,33 +220,44 @@ theorem VLCtx.IsDefEq.bind_lookup_eq_none (H : VLCtx.IsDefEq env U Δ₁ Δ₂) 
   repeat rw [forall_comm, forall_comm (α := VLocalDecl)]; refine forall_congr' fun _ => ?_
   simp only [← Option.eq_none_iff_forall_not_mem, H.lookup_eq_none]
 
+theorem VLocalDecl.IsDefEq.wf : VLocalDecl.IsDefEq env U Γ d₁ d₂ → VLocalDecl.WF env U Γ d₁
+  | .vlam h3 => ⟨_, h3.hasType.1⟩
+  | .vlet h3 _ => h3.hasType.1
+
 theorem VLCtx.IsDefEq.wf : VLCtx.IsDefEq env U Δ₁ Δ₂ → VLCtx.WF env U Δ₁
   | .nil => ⟨⟩
-  | .vlam h1 h2 h3 => ⟨h1.wf, h2, _, h3.hasType.1⟩
-  | .vlet h1 h2 h3 _ => ⟨h1.wf, h2, h3.hasType.1⟩
+  | .cons h1 h2 h3 => ⟨h1.wf, h2, h3.wf⟩
+
+theorem VLocalDecl.IsDefEq.symm :
+    VLocalDecl.IsDefEq env U Δ d₁ d₂ → VLocalDecl.IsDefEq env U Δ d₂ d₁
+  | .vlam h1 => .vlam h1.symm
+  | .vlet h1 h2 => .vlet (h2.defeqDF h1.symm) h2.symm
+
+theorem VLocalDecl.IsDefEq.defeqDFC (henv : Ordered env) (hΓ : IsDefEqCtx env U Γ₀ Γ₁ Γ₂)
+    : VLocalDecl.IsDefEq env U Γ₁ d₁ d₂ → VLocalDecl.IsDefEq env U Γ₂ d₁ d₂
+  | .vlam h1 => .vlam (h1.defeqDFC henv hΓ)
+  | .vlet h1 h2 => .vlet (h1.defeqDFC henv hΓ) (h2.defeqDFC henv hΓ)
 
 variable (henv : Ordered env) in
 theorem VLCtx.IsDefEq.symm : VLCtx.IsDefEq env U Δ₁ Δ₂ → VLCtx.IsDefEq env U Δ₂ Δ₁
   | .nil => .nil
-  | .vlam h1 h2 h3 =>
-    .vlam h1.symm (by simpa [h1.bind_lookup_eq_none] using h2) (h3.symm.defeqDFC henv h1.defeqCtx)
-  | .vlet h1 h2 h3 h4 =>
-    .vlet h1.symm (by simpa [h1.bind_lookup_eq_none] using h2)
-      (h4.defeqDF h3.symm |>.defeqDFC henv h1.defeqCtx) (h4.symm.defeqDFC henv h1.defeqCtx)
+  | .cons h1 h2 h3 =>
+    .cons h1.symm (by simpa [h1.bind_lookup_eq_none] using h2) (h3.symm.defeqDFC henv h1.defeqCtx)
 
 variable (henv : Ordered env) in
 theorem VLCtx.IsDefEq.find?_uniq (hΔ : VLCtx.IsDefEq env U Δ₁ Δ₂)
     (H1 : Δ₁.find? v = some (e₁, A₁)) (H2 : Δ₂.find? v = some (e₂, A₂)) :
     env.IsDefEqU U Δ₁.toCtx A₁ A₂ ∧ env.IsDefEq U Δ₁.toCtx e₁ e₂ A₁ := by
-  match hΔ with
-  | .vlam (type₁ := A₁) (type₂ := A₂) hΔ h2 h3 =>
+  let .cons hΔ h1 h2 := hΔ
+  match h2 with
+  | .vlam (type₁ := A₁) (type₂ := A₂) h2 =>
     revert H1 H2; unfold VLCtx.find?; split
-    · rintro ⟨⟩ ⟨⟩; exact ⟨⟨_, h3.weak henv⟩, .bvar .zero⟩
+    · rintro ⟨⟩ ⟨⟩; exact ⟨⟨_, h2.weak henv⟩, .bvar .zero⟩
     · simp [bind, Option.bind_eq_some]
       rintro ⟨d₁', n₁'⟩ H1' rfl rfl ⟨d₂', n₂'⟩ H2' rfl rfl
       obtain ⟨h2, h3⟩ := find?_uniq hΔ H1' H2'
       exact ⟨h2.weakN henv .one, h3.weak henv⟩
-  | .vlet hΔ _ h3 h4 =>
+  | .vlet h3 h4 =>
     revert H1 H2; unfold VLCtx.find?; split
     · rintro ⟨⟩ ⟨⟩; exact ⟨⟨_, h4⟩, h3⟩
     · simp [bind, Option.bind_eq_some]
@@ -129,22 +275,22 @@ theorem TrExpr.wf (H : TrExpr env Us Δ e e') : VExpr.WF env Us.length Δ.toCtx 
     simp [List.mapM_eq_some] at h2
     refine ⟨_, .const h1 (fun l hl => ?_) (h2.length_eq.symm.trans h3)⟩
     have ⟨_, _, h⟩ := h2.forall_exists_r _ hl; exact .of_ofLevel h
-  | app h1 h2 => exact ⟨_, .app h1 h2⟩
+  | app h1 h2 => exact ⟨_, h1.app h2⟩
   | lam h1 _ _ _ ih2 =>
     have ⟨_, h1'⟩ := h1
     have ⟨_, h2'⟩ := ih2 ⟨hΔ, rfl, h1⟩
-    refine ⟨_, .lam h1' h2'⟩
+    refine ⟨_, h1'.lam h2'⟩
   | forallE h1 h2 => have ⟨_, h1'⟩ := h1; have ⟨_, h2'⟩ := h2; exact ⟨_, .forallE h1' h2'⟩
   | letE h1 _ _ _ _ _ ih3 => exact ih3 ⟨hΔ, rfl, h1⟩
   | lit _ ih | mdata _ ih => exact ih hΔ
   | proj _ h2 ih => exact h2.wf (ih hΔ)
 
-variable (henv : Ordered env) (hΔ : VLCtx.IsDefEq env U Δ₁ Δ₂) in
-theorem TrProj.uniq (H1 : TrProj Δ₁ s i e₁ e₁') (H2 : TrProj Δ₂ s i e₂ e₂')
-    (H : env.IsDefEqU U Δ₁.toCtx e₁ e₂) :
-    env.IsDefEqU U Δ₁.toCtx e₁' e₂' := sorry
+variable (henv : Ordered env) (hΓ : IsDefEqCtx env U [] Γ₁ Γ₂) in
+theorem TrProj.uniq (H1 : TrProj Γ₁ s i e₁ e₁') (H2 : TrProj Γ₂ s i e₂ e₂')
+    (H : env.IsDefEqU U Γ₁ e₁ e₂) :
+    env.IsDefEqU U Γ₁ e₁' e₂' := sorry
 
-variable (henv : Ordered env) (Us : List Name) (hΔ : VLCtx.IsDefEq env Us.length Δ₁ Δ₂) in
+variable (henv : Ordered env) {Us : List Name} (hΔ : VLCtx.IsDefEq env Us.length Δ₁ Δ₂) in
 theorem TrExpr.uniq (H1 : TrExpr env Us Δ₁ e e₁) (H2 : TrExpr env Us Δ₂ e e₂) :
     env.IsDefEqU Us.length Δ₁.toCtx e₁ e₂ := by
   induction H1 generalizing Δ₂ e₂ with
@@ -162,18 +308,97 @@ theorem TrExpr.uniq (H1 : TrExpr env Us Δ₁ e e₁) (H2 : TrExpr env Us Δ₂ 
   | lam l1 _ _ ih2 ih3 =>
     let ⟨_, l1⟩ := l1; let .lam _ r2 r3 := H2
     have hA := ih2 hΔ r2 |>.of_l henv hΔ.wf.toCtx l1
-    have ⟨_, hb⟩ := ih3 (hΔ.vlam rfl hA) r3
+    have ⟨_, hb⟩ := ih3 (hΔ.cons rfl <| .vlam hA) r3
     exact ⟨_, .lamDF hA hb⟩
   | forallE l1 l2 _ _ ih3 ih4 =>
     let ⟨_, l1'⟩ := l1; let ⟨_, l2⟩ := l2; let .forallE _ _ r3 r4 := H2
     have hA := ih3 hΔ r3 |>.of_l henv hΔ.wf.toCtx l1'
-    have hB := ih4 (.vlam hΔ rfl hA) r4 |>.of_l (Γ := _::_) henv ⟨hΔ.wf.toCtx, l1⟩ l2
+    have hB := ih4 (hΔ.cons rfl (.vlam hA)) r4 |>.of_l (Γ := _::_) henv ⟨hΔ.wf.toCtx, l1⟩ l2
     exact ⟨_, .forallEDF hA hB⟩
   | letE l1 _ _ _ ih2 ih3 ih4 =>
     have hΓ := hΔ.wf.toCtx
     let .letE _ r2 r3 r4 := H2
     have ⟨_, hb⟩ := l1.isType henv hΓ
-    exact ih4 (.vlet hΔ rfl (ih3 hΔ r3 |>.of_l henv hΓ l1) (ih2 hΔ r2 |>.of_l henv hΓ hb)) r4
+    refine ih4 (hΔ.cons rfl ?_) r4
+    exact .vlet (ih3 hΔ r3 |>.of_l henv hΓ l1) (ih2 hΔ r2 |>.of_l henv hΓ hb)
   | lit _ ih1 => let .lit r1 := H2; exact ih1 hΔ r1
   | mdata _ ih1 => let .mdata r1 := H2; exact ih1 hΔ r1
   | proj _ l2 ih1 => let .proj r1 r2 := H2; exact l2.uniq r2 (ih1 hΔ r1)
+
+theorem TrExpr.weakN_inv (henv : Ordered env)
+    (W : VLCtx.LiftN Δ Δ₂ dk n k) (hΔ : VLCtx.IsDefEq env Us.length Δ₁ Δ₂)
+    (H : TrExpr env Us Δ₁ e e') (hs : InScope (· ∈ VLCtx.fvars Δ) e dk) :
+    ∃ e', TrExpr env Us Δ e e' := by
+  induction H generalizing Δ Δ₂ dk k with
+  | @bvar e A Δ₁ i h1 =>
+    suffices ∃ p, Δ.find? (.inl i) = some p from let ⟨_, h⟩ := this; ⟨_, .bvar h⟩
+    simp [InScope] at hs
+    induction W generalizing i e A Δ₁ with | @cons_bvar _ Δ₂ _ _ _ d W ih => ?_ | _ => cases hs
+    obtain ⟨d, Δ₂, rfl, hΔ₁⟩ : ∃ d Δ₁', Δ₁ = (none, d) :: Δ₁' ∧
+        VLCtx.IsDefEq env Us.length Δ₁' Δ₂ := by cases d <;> cases hΔ <;> exact ⟨_, _, rfl, ‹_›⟩
+    simp [VLCtx.find?] at h1 ⊢
+    rcases i with _ | i <;> simp [VLCtx.next, bind] at h1 ⊢
+    obtain ⟨_, h1, _⟩ := h1
+    have ⟨_, h1⟩ := ih h1 hΔ₁ (Nat.lt_of_succ_lt_succ hs)
+    exact ⟨_, _, h1, rfl⟩
+  | @fvar e A _ fv h1 =>
+    simp [InScope, VLCtx.mem_fvars, ← Option.isSome_iff_exists, VLCtx.lookup_isSome] at hs
+    let ⟨_, h⟩ := Option.isSome_iff_exists.1 hs
+    exact ⟨_, .fvar h⟩
+  | sort h1 => exact ⟨_, .sort h1⟩
+  | const h1 h2 h3 => exact ⟨_, .const h1 h2 h3⟩
+  | app h1 h2 hf ha ih1 ih2 =>
+    have hΔ₁ := hΔ.wf; have hΔ₂ := (hΔ.symm henv).wf
+    let ⟨f₁, ih1⟩ := ih1 W hΔ hs.1
+    let ⟨a₁, ih2⟩ := ih2 W hΔ hs.2
+    have h1 := h1.defeqU_l henv hΔ₁.toCtx <| hf.uniq henv hΔ (ih1.weakN henv W hΔ₂)
+    have h2 := h2.defeqU_l henv hΔ₁.toCtx <| ha.uniq henv hΔ (ih2.weakN henv W hΔ₂)
+    have := VExpr.WF.weakN_iff henv hΔ₂.toCtx W.toCtx (e := f₁.app a₁)
+    have := this.1 ⟨_, (h1.app h2).defeqDFC henv hΔ.defeqCtx⟩
+    have ⟨_, _, h1, h2⟩ := this.app_inv henv (W.wf henv hΔ₂).toCtx
+    exact ⟨_, .app h1 h2 ih1 ih2⟩
+  | lam h1 ht hb ih1 ih2 =>
+    let ⟨_, h1⟩ := h1
+    have hΔ₁ := hΔ.wf; have hΔ₂ := (hΔ.symm henv).wf
+    let ⟨ty₁, ih1⟩ := ih1 W hΔ hs.1
+    have htt := ht.uniq henv hΔ (ih1.weakN henv W hΔ₂) |>.of_l henv hΔ₁.toCtx h1
+    have ⟨_, ih2⟩ := ih2 (W.cons_bvar (.vlam _))
+      (hΔ.cons (ofv := none) rfl <| .vlam htt) hs.2.fvars_cons
+    have h1 := HasType.weakN_iff (A := .sort _) henv hΔ₂.toCtx W.toCtx
+      |>.1 (htt.hasType.2.defeqDFC henv hΔ.defeqCtx)
+    exact ⟨_, .lam ⟨_, h1⟩ ih1 ih2⟩
+  | forallE h1 h2 ht hb ih1 ih2 =>
+    let ⟨_, h1⟩ := h1; let ⟨_, h2⟩ := h2
+    have hΔ₁ := hΔ.wf; have hΔ₂ := (hΔ.symm henv).wf
+    let ⟨ty₁, ih1⟩ := ih1 W hΔ hs.1
+    have htt := ht.uniq henv hΔ (ih1.weakN henv W hΔ₂) |>.of_l henv hΔ₁.toCtx h1
+    have hΔ' := hΔ.cons (ofv := none) rfl <| .vlam htt
+    have ⟨_, ih2⟩ := ih2 (W.cons_bvar (.vlam _)) hΔ' hs.2.fvars_cons
+    have h1' := htt.hasType.2.defeqDFC henv hΔ.defeqCtx
+    have h1 := HasType.weakN_iff (A := .sort _) henv hΔ₂.toCtx W.toCtx |>.1 h1'
+    have hΔ₂' : VLCtx.WF _ _ ((none, .vlam _) :: _) := ⟨hΔ₂, rfl, _, h1'⟩
+    have h2 := (HasType.weakN_iff (A := .sort _) henv hΔ₂'.toCtx (W.cons_bvar (.vlam _)).toCtx).1 <|
+      hb.uniq henv hΔ' (ih2.weakN henv (W.cons_bvar _) hΔ₂')
+      |>.of_l (Γ := _::_) henv ⟨hΔ₁.toCtx, _, htt.hasType.1⟩ h2
+      |>.hasType.2.defeqDFC henv (.succ hΔ.defeqCtx htt)
+    exact ⟨_, .forallE ⟨_, h1⟩ ⟨_, h2⟩ ih1 ih2⟩
+  | letE h1 ht hv hb ih1 ih2 ih3 =>
+    have hΔ₁ := hΔ.wf; have hΔ₂ := (hΔ.symm henv).wf
+    let ⟨ty₁, ih1⟩ := ih1 W hΔ hs.1
+    let ⟨val₁, ih2⟩ := ih2 W hΔ hs.2.1
+    have hvv := hv.uniq henv hΔ (ih2.weakN henv W hΔ₂) |>.of_l henv hΔ₁.toCtx h1
+    let ⟨_, h2⟩ := h1.isType henv hΔ₁.toCtx
+    have htt := ht.uniq henv hΔ (ih1.weakN henv W hΔ₂) |>.of_l henv hΔ₁.toCtx h2
+    have ⟨_, ih3⟩ := ih3 (W.cons_bvar (.vlet ..)) (hΔ.cons rfl <| .vlet hvv htt) hs.2.2.fvars_cons
+    have h1 := HasType.weakN_iff henv hΔ₂.toCtx W.toCtx
+      |>.1 ((htt.defeqDF hvv).hasType.2.defeqDFC henv hΔ.defeqCtx)
+    exact ⟨_, .letE h1 ih1 ih2 ih3⟩
+  | lit _ ih => let ⟨_, ih⟩ := ih W hΔ .toConstructor; exact ⟨_, .lit ih⟩
+  | mdata _ ih => let ⟨_, ih⟩ := ih W hΔ hs; exact ⟨_, .mdata ih⟩
+  | proj h1 h2 ih =>
+    have hΔ₁ := hΔ.wf; have hΔ₂ := (hΔ.symm henv).wf
+    let ⟨_, ih⟩ := ih W hΔ hs
+    have htt := h1.uniq henv hΔ (ih.weakN henv W hΔ₂)
+    have ⟨_, h2⟩ := h2.defeqDFC henv hΔ.defeqCtx htt
+    have ⟨_, h2⟩ := h2.weakN_inv henv hΔ₂.toCtx W.toCtx
+    exact ⟨_, .proj ih h2⟩
