Lean4Lean/Verify/Typing/LocalContext.lean
@@ -12,25 +12,10 @@ theorem ConditionallyTyped.mono (H : ngen₁ ≤ ngen₂) :
     ConditionallyTyped ngen₁ env Us Δ e → ConditionallyTyped ngen₂ env Us Δ e
   | ⟨h1, h2⟩ => ⟨h1.mono fun _ h => h.mono H, h2⟩
 
-theorem ConditionallyTyped.liftN_inv
-    (H : ConditionallyTyped ngen env Us (d :: Δ) e) : ConditionallyTyped ngen env Us Δ e := by
+theorem ConditionallyTyped.weakN_inv
+    (henv : Ordered env) (hΔ : VLCtx.WF env Us.length ((some fv, d) :: Δ))
+    (H : ConditionallyTyped ngen env Us ((some fv, d) :: Δ) e) :
+    ConditionallyTyped ngen env Us Δ e := by
   refine H.imp_right fun H1 H2 => ?_
-  have ⟨e', H⟩ := H1 <| H2.mono fun _ h => by
-    simp [VLCtx.fvars]; split <;> [exact h; exact h.tail _]
-  sorry
-  -- induction H with
-  -- | bvar h1 | fvar h1 => exact ⟨_, hΔ.find?_wf henv h1⟩
-  -- | sort h1 => exact ⟨_, .sort (.of_ofLevel h1)⟩
-  -- | const h1 h2 h3 =>
-  --   simp [List.mapM_eq_some] at h2
-  --   refine ⟨_, .const h1 (fun l hl => ?_) (h2.length_eq.symm.trans h3)⟩
-  --   have ⟨_, _, h⟩ := h2.forall_exists_r _ hl; exact .of_ofLevel h
-  -- | app h1 h2 => exact ⟨_, .app h1 h2⟩
-  -- | lam h1 _ _ _ ih2 =>
-  --   have ⟨_, h1'⟩ := h1
-  --   have ⟨_, h2'⟩ := ih2 ⟨hΔ, rfl, h1⟩
-  --   refine ⟨_, .lam h1' h2'⟩
-  -- | forallE h1 h2 => have ⟨_, h1'⟩ := h1; have ⟨_, h2'⟩ := h2; exact ⟨_, .forallE h1' h2'⟩
-  -- | letE h1 _ _ _ _ _ ih3 => exact ih3 ⟨hΔ, rfl, h1⟩
-  -- | lit _ ih | mdata _ ih => exact ih hΔ
-  -- | proj _ h2 ih => exact h2.wf (ih hΔ)
+  have ⟨e', H⟩ := H1 H2.fvars_cons
+  exact TrExpr.weakN_inv henv (.skip_fvar _ _ .refl) (.refl henv hΔ) H H2
